add choice nodes

simpleversionTree.dfy
@@ -1,65 +1,154 @@
+datatype NodeType =
+  Normal | Choice
+
 datatype FoodTree =
-  FoodNode(name: string, children: seq<FoodTree>)
+  FoodNode(name: string, nodeType: NodeType, children: seq<FoodTree>)
+
+datatype FoodLabel =
+  Safe | Warning | Unsafe
 
 datatype LabeledTree = 
-  LabeledNode(name: string, labelname: string, children: seq<LabeledTree>)
+  LabeledNode(name: string, labelname: FoodLabel, children: seq<LabeledTree>)
 
-predicate AllergenFree(t: FoodTree, allergens: set<string>) {
-  !(t.name in allergens) && forall child :: child in t.children ==> AllergenFree(child, allergens)
+predicate IsSafe(t: FoodTree, allergens: set<string>) {
+  // "safe" indicates that the node is completely allergen-free
+  AllSafe(t, allergens) && SomeSafe(t, allergens)
+}
+predicate IsWarning(t: FoodTree, allergens: set<string>) {
+  // "warning" indicates the node has allergen free options available (but not all options are allergen tree)
+  SomeSafe(t, allergens) && !AllSafe(t, allergens)
+}
+predicate IsUnsafe(t: FoodTree, allergens: set<string>) {
+  // "unsafe" idicates the node is guarenteed to contain the allergen (all options contain the allergen)
+  !SomeSafe(t, allergens) && !AllSafe(t, allergens)
+}
+
+predicate AllSafe(t: FoodTree, allergens: set<string>) {
+  !(t.name in allergens) && forall child :: child in t.children ==> AllSafe(child, allergens)
+}
+predicate SomeSafe(t: FoodTree, allergens: set<string>) {
+  AllSafe(t, allergens) || (
+  !(t.name in allergens) && 
+  match t.nodeType
+  case Normal =>
+    forall child :: child in t.children ==> SomeSafe(child, allergens)
+  case Choice =>
+    // Check to see if at least one option is safe
+    |t.children| == 0 || exists child :: child in t.children && SomeSafe(child, allergens))
+}
+
+predicate NodeCorrect(t: FoodTree, lt: LabeledTree, allergens: set<string>) {
+  // Check that for the root node in the label tree:
+  // 1. Has a name that matches the original food tree
+  lt.name == t.name &&
+  // 2. The children's lengths are equivalent
+  |lt.children| == |t.children| &&
+  // 3. Label is correct
+  (lt.labelname == Safe <==> IsSafe(t, allergens)) && 
+  (lt.labelname == Warning <==> IsWarning(t, allergens)) &&
+  (lt.labelname == Unsafe <==> IsUnsafe(t, allergens))
 }
 
 predicate AllNodesCorrect(t: FoodTree, lt: LabeledTree, allergens: set<string>)
 {
-  // Check that for all nodes in the label tree:
-  // 1. Has a name that match the original food tree
-  lt.name == t.name &&
-  // 2. Label is correct ("safe" indicates the node is alergen free)
-  (lt.labelname == "safe" <==> AllergenFree(t, allergens)) &&
-  // 3. The children's lengths are equivalent
-  |lt.children| == |t.children| &&
-  // 4. All children are also correct
+  NodeCorrect(t, lt, allergens) &&
+  // 4. All children are also correct (matching name/children lengths and correct label)
   forall i: nat :: 0 <= i < |t.children| ==> AllNodesCorrect(t.children[i], lt.children[i], allergens)
 }
 
 method LabelTree(t: FoodTree, allergens: set<string>) returns (lt: LabeledTree)
   ensures lt.name == t.name
   ensures |lt.children| == |t.children|
-  ensures lt.labelname in {"safe", "not safe"}
-  ensures AllNodesCorrect(t, lt, allergens)
+  ensures lt.labelname == Safe <==> IsSafe(t, allergens)
+  ensures lt.labelname == Warning <==> IsWarning(t, allergens)
+  ensures lt.labelname == Unsafe <==> IsUnsafe(t, allergens)
+  //ensures AllNodesCorrect(t, lt, allergens)
 {
   var name := t.name;
   var children := t.children;
 
   var labeledChildren: seq<LabeledTree> := [];
   ghost var processedChildren: seq<FoodTree> := [];
-  var anyUnsafe := false;
 
-  if name in allergens {
-    anyUnsafe := true;
-  }
+  var isAllergen := name in allergens;
+  var noChildren := |children| == 0;
+
+  // Initialize basebases
+  var existsSomeSafe := false;
+  var allSomeSafe := true;
+  var allSafe := true;
+  assert allSafe == allSomeSafe;
   var i := 0;
   while i < |children|
     invariant 0 <= i <= |children|
     invariant |labeledChildren| == |processedChildren| == i
     invariant forall i: nat :: 0 <= i < |processedChildren| ==> processedChildren[i] == children[i]
     invariant forall i: nat :: 0 < i < |processedChildren| ==> labeledChildren[i].name == processedChildren[i].name
-    invariant forall i: nat :: 0 <= i < |processedChildren| ==> AllNodesCorrect(processedChildren[i], labeledChildren[i], allergens)    
-    invariant !anyUnsafe <==> !(name in allergens) && forall child :: child in processedChildren ==> AllergenFree(child, allergens)
+    //invariant forall i: nat :: 0 <= i < |processedChildren| ==> AllNodesCorrect(processedChildren[i], labeledChildren[i], allergens)    
+    invariant existsSomeSafe <==> exists child :: child in processedChildren && SomeSafe(child, allergens)
+    invariant allSomeSafe <==> forall child :: child in processedChildren ==> SomeSafe(child, allergens)
+    invariant allSafe <==> forall child :: child in processedChildren ==> AllSafe(child, allergens)
+    invariant allSafe ==> allSomeSafe
     decreases |children| - i
   {
     var child := children[i];
     var childLabeled := LabelTree(child, allergens);
-    assert childLabeled.labelname == "safe" <==> AllergenFree(child, allergens);
-    if childLabeled.labelname == "not safe" {
-      anyUnsafe := true;
+    assert NodeCorrect(child, childLabeled, allergens);
+    if childLabeled.labelname == Unsafe {
+      assert !SomeSafe(child, allergens);
+      assert !AllSafe(child, allergens);
+      allSafe := false;
+      allSomeSafe := false;
+    } else if childLabeled.labelname == Warning {
+      assert SomeSafe(child, allergens);
+      assert !AllSafe(child, allergens);
+      existsSomeSafe := true;
+      allSafe := false;
+    } else {
+      assert childLabeled.labelname == Safe;
+      assert SomeSafe(child, allergens);
+      assert AllSafe(child, allergens);
+      existsSomeSafe := true;
     }
     labeledChildren := labeledChildren + [childLabeled];
     processedChildren := processedChildren + [child];
     i := i + 1;
   }
-  assert anyUnsafe <==> name in allergens || !(forall child :: child in processedChildren ==> AllergenFree(child, allergens));
-  assert anyUnsafe <==> !AllergenFree(t, allergens);
-  var labelN := if anyUnsafe then "not safe" else "safe";
+  assert children == processedChildren;
+  assert existsSomeSafe <==> exists child :: child in children && SomeSafe(child, allergens);
+  assert allSomeSafe <==> forall child :: child in children ==> SomeSafe(child, allergens);
+  assert allSafe <==> forall child :: child in children ==> AllSafe(child, allergens);
+  
+  ghost var fullAllSafe := !isAllergen && allSafe;
+  ghost var fullSomeSafe := fullAllSafe || ( !isAllergen && match t.nodeType
+            case Normal => allSomeSafe
+            case Choice => noChildren || existsSomeSafe );
+  assert fullAllSafe <==> AllSafe(t, allergens);
+  assert fullSomeSafe <==> SomeSafe(t, allergens);
+  
+  ghost var isSafe := fullAllSafe && fullSomeSafe;
+  ghost var isWarning := fullSomeSafe && !fullAllSafe;
+  ghost var isUnsafe := !fullSomeSafe && !fullAllSafe;
+  assert isWarning <==> IsWarning(t, allergens);
+  assert isSafe <==> IsSafe(t, allergens);
+  assert isUnsafe <==> IsUnsafe(t, allergens);
+
+  var labelN :=
+    if isAllergen then
+      Unsafe
+    else if allSafe then
+      Safe
+    else if (match t.nodeType
+             case Normal => allSomeSafe
+             case Choice => noChildren || existsSomeSafe) then
+      Warning
+    else
+      Unsafe;
+
+  assert labelN == Safe <==> isSafe;
+  assert labelN == Warning <==> isWarning;
+  assert labelN == Unsafe <==> isUnsafe;
+
   lt := LabeledNode(name, labelN, labeledChildren);
 }
 
@@ -72,7 +161,11 @@ function Pad(n: nat): string
 method PrintLabeledTree(t: LabeledTree, indent: nat)
 {
   var pad := Pad(indent);
-  print pad + t.name + " (" + t.labelname + ")\n";
+  var labelStr := match t.labelname
+    case Safe => "Safe"
+    case Warning => "Warning: Some options are unsafe"
+    case Unsafe => "Unsafe";
+  print pad + t.name + " (" + labelStr + ")" + "\n";
   var i := 0;
   while i < |t.children|
     decreases |t.children| - i
@@ -82,22 +175,37 @@ method PrintLabeledTree(t: LabeledTree, indent: nat)
   }
 }
 
+function Ingredient(name: string): FoodTree {
+  FoodNode(name, Normal, [])
+}
+
+function Recipe(name: string, children: seq<FoodTree>): FoodTree {
+  FoodNode(name, Normal, children)
+}
+
+function ChooseOne(name: string, children: seq<FoodTree>): FoodTree {
+  FoodNode(name + " (choose one)", Choice, children)
+}
+
 method Main()
 {
-  var flour := FoodNode("flour", []);
-  var lactose := FoodNode("lactose", []);
-  var milk := FoodNode("milk", [lactose]);
-  var tortila := FoodNode("tortila", [flour, milk]);
-  var bread := FoodNode("bread", [flour, tortila]);
+  var flour := Ingredient("flour");
+  var lactose := Ingredient("lactose");
+  var milk := Recipe("milk", [lactose]);
+  var tortila := Recipe("tortila", [flour, milk]);
+  var bread := Recipe("bread", [flour, tortila]);
 
-  var chicken := FoodNode("chicken", []);
-  var letus := FoodNode("letus", []);
-  var tomato := FoodNode("tomato", []);
-  var salad := FoodNode("salad", [letus, tomato]);
+  var chicken := Ingredient("chicken");
+  var ham := Ingredient("ham");
+  var protein := ChooseOne("Protein Topping", [chicken, ham]);
 
-  var sandwich := FoodNode("sandwich", [bread, chicken, salad]);
+  var letus := Ingredient("letus");
+  var tomato := Ingredient("tomato");
+  var salad := Recipe("salad", [letus, tomato]);
 
-  var allergens := { "tortila", "tomato", "lactose" };
+  var sandwich := Recipe("sandwich", [bread, protein, salad]);
+
+  var allergens := { "tortila", "tomato", "lactose", "ham"};
 
   var labeled := LabelTree(sandwich, allergens);
 
